src/program_proof/session/maxTS/proof.v
@@ -1,0 +1,73 @@
+From Goose.github_com.session Require Import maxTS.
+From Perennial.program_proof Require Import std_proof. 
+From Perennial.goose_lang.ffi.grove_ffi Require Export impl.
+From Perennial.program_logic Require Export atomic.
+From Perennial.program_proof Require Export proof_prelude.
+From Perennial.program_proof Require Import grove_prelude.
+From Perennial.goose_lang.lib Require Import struct.struct into_val.
+From RecordUpdate Require Import RecordSet.
+From Perennial.goose_lang Require Import prelude.
+
+Local Lemma Z_scope_test : (0%Z) + (0%Z) = 0%Z.
+Proof. done. Qed.
+
+Section heap.
+  
+  Context `{hG: !heapGS Σ}.
+
+  Definition coqMax (x: w64) (y: w64) :=
+    if uint.Z x >? uint.Z y then x else y. 
+
+  Fixpoint maxTSCoq (t1: list w64) (t2: list w64) : list w64 :=
+    match t1 with
+    | [] => []
+    | cons hd1 tl1 => match t2 with
+                      | [] => [] (* this shouldn't happen*)
+                      | cons hd2 tl2 => if (uint.Z hd1) >? (uint.Z hd2) then
+                                          (cons hd1 (maxTSCoq tl1 tl2)) else (cons hd2 (maxTSCoq tl1 tl2))
+                      end
+    end.
+
+  Lemma max_equiv (x: w64) (y: w64) :
+    {{{
+          True
+    }}}
+      maxTwoInts #x #y 
+      {{{
+            r , RET #r;
+            ⌜r = coqMax x y⌝
+      }}}.
+  Proof.
+    iIntros (Φ) "H H1".
+    unfold maxTwoInts. wp_pures.
+    wp_if_destruct.
+    - iModIntro. iApply "H1". iPureIntro.
+      unfold coqMax. apply Z.gtb_lt in Heqb.
+      rewrite Heqb. auto.
+    - iModIntro. iApply "H1". iPureIntro.
+      unfold coqMax.
+      assert (uint.Z y >= uint.Z x) by word.
+      assert (uint.Z x >? uint.Z y = false) by word.
+      rewrite H0.
+      auto.
+  Qed.
+
+  (* Lemma getMaxTsEquiv (x: Slice.t) (xs: list w64) (y: Slice.t) (ys: list w64) :
+    {{{
+          own_slice x uint64T (DfracOwn 1) xs ∗
+          own_slice y uint64T (DfracOwn 1) ys 
+    }}}
+      maxTS x y 
+      {{{
+            (r: Slice.t), RET slice_val r;
+            own_slice r uint64T (DfracOwn 1) (maxTSCoq xs ys) ∗ (* what is slice_val? *)
+            own_slice x uint64T (DfracOwn 1) xs ∗
+            own_slice y uint64T (DfracOwn 1) ys 
+      }}}.
+  Proof.
+    iIntros (Φ) "H H1".
+    unfold maxTS.
+    wp_pures. wp_apply wp_ref_to. *)
+    
+    
+End heap.
